examples/ecAdd/proofs/ecAdd.ec
@@ -4,495 +4,111 @@ require import Gcd Gcd_props.
 require import AlmostYUL.
 require import Montgomery_arith.
 
-
-op pointIsInCurve (x y : int) = (y * y) %% P = (x * x * x + 3) %% P.
-
-
-lemma pointIsInCurve_m_h (x_in y_in : int) :
- hoare [ AlmostYul.pointIsInCurve : arg = (x_in * R %% P, y_in * R %% P) ==>  
-       res = (y_in * y_in * R %% P = (x_in * x_in * x_in * R + 3 * R) %% P ) ].
-admitted.
+require import EcAdd_cases EcAdd_functions.
 
 
+(* lemma ecAdd_correctness2  (x1_in y1_in x2_in y2_in : int) : *)
+(*              !(x1_in < P *)
+(*          /\ y1_in < P *)
+(*          /\  x2_in < P *)
+(*          /\  y2_in < P *)
+(*          /\ (!pIsInfinity (x1_in, y1_in) => pointIsInCurve x1_in y1_in) *)
+(*          /\ (!pIsInfinity (x2_in, y2_in) => pointIsInCurve x2_in y2_in)) = *)
+    
+(*             (P <= x1_in *)
+(*          \/  P <= y1_in *)
+(*          \/  P <= x2_in  *)
+(*          \/  P <= y2_in) *)
+            
+(*          \/ ((!pIsInfinity (x1_in, y1_in) /\ !pointIsInCurve x1_in y1_in) *)
+(*          \/ (!pIsInfinity (x2_in, y2_in) /\ !pointIsInCurve x2_in y2_in)). *)
 
-lemma ecAdd_correct_1 x1_in y1_in x2_in y2_in :  
- phoare[ AlmostYul.main : 
-         arg = (x1_in,y1_in,x2_in,y2_in)  
-         /\ (x1_in = 0 /\ y1_in = 0) 
-         /\ (x2_in = 0 /\ y2_in = 0)
-                 ==> res = (0,0) ] = 1%r.
-proc. 
-rcondt 5. inline*. wp. skip. progress. 
-rcondf 7. inline*. wp. skip. progress.
-inline*. wp. auto. qed.
+(* smt(). *)
+(* qed. *)
+            
+lemma ecAdd_correctness2  (x1_in y1_in x2_in y2_in : int) :    
+          
+       !((P <= x1_in
+         \/  P <= y1_in
+         \/  P <= x2_in 
+         \/  P <= y2_in) /\ 
 
+         ((!pIsInfinity (x1_in, y1_in) /\ !pointIsInCurve x1_in y1_in)
+            \/ (!pIsInfinity (x2_in, y2_in) /\ !pointIsInCurve x2_in y2_in))).
 
-lemma ecAdd_correct_2 x1_in y1_in x2_in y2_in :  
- hoare[ AlmostYul.main : 
-         arg = (x1_in,y1_in,x2_in,y2_in)  
-         /\ (x1_in = 0 /\ y1_in = 0) 
-         /\ !(x2_in = 0 /\ y2_in = 0)
-         /\ 0 <= x2_in < AlmostYUL.N 
-         /\ 0 <= y2_in < AlmostYUL.N
-         /\ pointIsInCurve x2_in y2_in  
-                  ==> res = (x2_in,y2_in) ].
-proc. 
-rcondf 5. inline*. wp. skip. progress. 
-rcondt 5. inline*. wp. skip. progress.
-rcondf 8. inline*. auto. sp. if. wp. sp.  auto. skip. smt().
-rcondt 7. inline*. wp. skip. progress.
-rcondf 12. inline*. wp. skip. progress.           smt().
-seq 13 : (#pre /\ m_x2 = x2_in * R %% P  /\ m_y2 = y2_in * R %% P). auto.
-ecall (into_m_h y2).
-ecall (into_m_h x2).
-inline*. auto.           
-wp.
-rcondf 3. 
-inline AlmostYul.iszero. wp.
-ecall (pointIsInCurve_m_h x2 y2). skip. progress. rewrite /as_bool. simplify.
-rewrite /pointIsInCurve in H4.
- have ->: y2{hr} * y2{hr} * R %% P = y2{hr} * y2{hr} %% P * R %% P.
-  smt (@Int @IntDiv).                
-  rewrite H4. smt(@IntDiv).
-call (_:true);auto.
-call (_:true);auto.             
-qed.           
-
-
-lemma ecAdd_correct_3 x1_in y1_in x2_in y2_in :  
- hoare[ AlmostYul.main : 
-         arg = (x1_in,y1_in,x2_in,y2_in) 
-         /\ !(x1_in = 0 /\ y1_in = 0)
-         /\ (x2_in = 0 /\ y2_in = 0) 
-         /\ 0 <= x1_in < AlmostYUL.N 
-         /\ 0 <= y1_in < AlmostYUL.N
-         /\ pointIsInCurve x1_in y1_in 
-               ==> res = (x1_in,y1_in) ].
-proc. 
-rcondf 5. inline*. wp. skip. progress. 
-rcondt 5. inline*. wp. skip. progress. 
-rcondf 7. inline*. auto.
-rcondt 7. inline*. wp. skip. progress.
-rcondt 9. inline*. wp. skip. progress.       
-rcondf 22.  wp.  auto.
-rcondf 14. inline*. wp. skip. progress.        smt().
-seq 15 : (#pre /\ m_x1 = x1_in * R %% P  /\ m_y1 = y1_in * R %% P). auto.
-ecall (into_m_h y1).
-ecall (into_m_h x1).
-inline*. auto.
-wp. rcondf 3.       
-inline AlmostYul.iszero. wp.
-ecall (pointIsInCurve_m_h x1 y1). skip. progress. rewrite /as_bool. simplify.
-rewrite /pointIsInCurve in H4.
-have ->: y1{hr} * y1{hr} * R %% P
-  = y1{hr} * y1{hr} %% P * R %% P. smt(@IntDiv).
-rewrite H4. smt(@IntDiv).
-call (_:true);auto.
-call (_:true);auto.
-qed.       
-
-lemma ecAdd_correct_4 x1_in y1_in x2_in y2_in :  
- hoare[ AlmostYul.main : 
-         arg = (x1_in,y1_in,x2_in,y2_in) 
-         /\ !(x1_in = 0 /\ y1_in = 0)
-         /\ !(x2_in = 0 /\ y2_in = 0) 
-         /\ 0 <= x1_in < AlmostYUL.N 
-         /\ 0 <= y1_in < AlmostYUL.N
-         /\ 0 <= x2_in < AlmostYUL.N 
-         /\ 0 <= y2_in < AlmostYUL.N      
-         /\ pointIsInCurve x1_in y1_in
-         /\ pointIsInCurve x2_in y2_in
-         /\ x1_in = x2_in /\ (P - y1_in) %% P = y2
-               ==> res = (0,0) ].
-proc.             
-rcondf 5. inline*. wp. skip. progress.  smt().
-rcondt 5. inline*. wp. skip. progress. 
-rcondf 7. inline*. auto. smt().
-rcondt 7. inline*. wp. skip. progress.
-rcondf 9. inline*. wp. skip. progress. smt().
-rcondt 9. inline*. auto. 
-rcondf 14. inline*. auto. smt().
-rcondf 19. inline*. auto. smt().
-rcondt 24. inline*. auto. progress. rewrite /as_bool. smt.
-rcondf 36. wp. auto.
-wp.
-seq 27 : (#pre /\ m_x1 = x1_in * R %% P  
-               /\ m_y1 = y1_in * R %% P 
-               /\ m_x2 = x2_in * R %% P  
-               /\ m_y2 = y2_in * R %% P). auto.
-ecall (into_m_h y2).
-ecall (into_m_h x2).
-ecall (into_m_h y1).
-ecall (into_m_h x1).
-inline*. auto. progress.  qed.
-
-
-lemma nosmt div_fact (a P : int) : 0 < a < P /\ 0 <= P => !(P %| a).
-progress. smt(@Int @IntDiv dvdn_le). qed.
-
-
-
-lemma nosmt div_fact2 (a P : int) : 1 < P => coprime P a => !(P %| a).
-progress.
-have ->: a = a * 1. smt().
-case (P %| a * 1);auto.
-move => q.
-have : P %| 1.
-    apply (Gauss P a 1).     auto. auto.
-apply div_fact. progress. smt().
-qed.    
-
-
-lemma qqq (a b P : int) : (a - b) %% P = (a %% P - b %% P) %% P.
-    smt(@Int @IntDiv). qed.
-
-search (%|).
-lemma nosmt oi (y1 y2 : int) : 0 <= y1 < P /\ 0 <= y2 < P => y1 <> y2 => 0 < y1 + y2 => y1^2 %% P = y2^2 %% P => y1 %% P = (P - y2) %% P.
-progress.
-have fact1 : y1^2 %% P - y2^2 %% P = 0.    smt.
-have  :  (y1^2  - y2^2) %% P  = 0. rewrite qqq. rewrite fact1. auto.
-have  ->:  (y1^2  - y2^2) = (y1 - y2) * (y1 + y2). smt.
-progress.
-rewrite - dvdzE in H6.
-have fact2 : P %| (y1 + y2). apply (Gauss P _ _ H6).
-apply prime_coprime. smt. 
-have : `|y1 - y2| < P. smt(@Int).
-progress.
-case ((y1 - y2) %% P = 0). 
-move => oo.
-have : `|y1 - y2| %% P = 0. smt (@Int @IntDiv).
-progress. apply div_fact2. smt. apply prime_coprime. smt. smt.
-auto.
-have fact4 : exists k, (y1 + y2) = k * P.
-     have d :   P %| (y1 + y2) <=> exists (q : int), y1 + y2 = q * P. apply (dvdzP P (y1 + y2)).
-       elim d. progress. apply (H7 fact2).
-elim fact4. progress.
-have o1 : k = 1. smt.
-have : P = y1 + y2. smt.
-smt.
-qed.
-
-
-
-op add_x' (x1 x2 y1 y2 : int) =  let slope = (y2 - y1) * inv P (x2 - x1) in (slope * slope - (x1 + x2)).
-op add_y' (x1 x2 y1 y2 : int) =  let slope = (y2 - y1) * inv P (x2 - x1) in
-                           (slope * (x1 - (slope * slope - (x1 + x2))) - y1).
-
-lemma ecAdd_correct_6 x1_in y1_in x2_in y2_in :  
- hoare[ AlmostYul.main : 
-         arg = (x1_in,y1_in,x2_in,y2_in)
-         /\ 0 <= x1_in < AlmostYUL.N 
-         /\ 0 <= y1_in < AlmostYUL.N 
-         /\ 0 <= x2_in < AlmostYUL.N 
-         /\ 0 <= y2_in < AlmostYUL.N      
-         /\ pointIsInCurve x1_in y1_in
-         /\ pointIsInCurve x2_in y2_in
-
-         /\ !(x1_in = 0 /\ y1_in = 0)
-         /\ !(x2_in = 0 /\ y2_in = 0) 
-         /\ !(x1_in = x2_in /\ y1_in = y2_in)
-         /\ !(x1_in = x2_in /\ (P - y1_in) %% P = y2)
-               ==> res = (add_x' x1_in x2_in y1_in y2_in %% P, add_y' x1_in x2_in y1_in y2_in %% P) ].
-proc.             
-rcondf 5. inline*. wp. skip. progress. smt().
-rcondt 5. inline*. wp. skip. progress. 
-rcondf 7. inline*. auto. smt().
-rcondt 7. inline*. wp. skip. progress.
-rcondf 9. inline*. wp. skip. progress. smt().
-rcondt 9. inline*. auto. 
-rcondf 14. inline*. auto. smt().
-rcondf 19. inline*. auto. smt().
-rcondf 24. inline*. auto. progress. rewrite /as_bool.
- have f: (AlmostYUL.N - y1{hr}) %% R = (AlmostYUL.N - y1{hr}). smt.
- rewrite f f. clear f.             
-case (x1{hr} = x2{hr}). progress.
-smt. auto.             
-rcondt 24. inline*. auto. progress. rewrite /as_bool.
-rcondf 37. inline*. auto.  progress. rewrite /as_bool.
-seq 90 : (#pre). wp. skip. auto.
-if.  while (true). auto.              auto.
-skip. progress.
-seq 36 : (#pre /\ ret_bool = false).             
-inline *. seq 90 : (#pre /\ ret_bool = false). wp. skip. auto.
-wp. if.  while (true). auto.              auto.
-skip. auto. progress.
-rcondt 1. auto.
-seq 4 : ((
-   (0 <= x1_in && x1_in < AlmostYUL.N) /\
-   (0 <= y1_in && y1_in < AlmostYUL.N) /\
-   (0 <= x2_in && x2_in < AlmostYUL.N) /\
-   (0 <= y2_in && y2_in < AlmostYUL.N) /\
-   pointIsInCurve x1_in y1_in /\
-   pointIsInCurve x2_in y2_in /\
-   ! (x1_in = 0 /\ y1_in = 0) /\
-   ! (x2_in = 0 /\ y2_in = 0) /\
-   ! (x1_in = x2_in /\ y1_in = y2_in) /\ ! (x1_in = x2_in /\ (P - y1_in) %% P = y2_in)) /\
-  ret_bool = false /\ x1 = x1_in * R %% P
-  /\ y1 = y1_in * R %% P
- /\ x2 = x2_in * R %% P
-/\ y2 = y2_in * R %% P).
-ecall (into_m_h y2_in). 
-ecall (into_m_h x2_in).
-ecall (into_m_h y1_in).                          
-ecall (into_m_h x1_in).
-skip. progress. 
-seq 6 : (#pre).
-seq 5 : (#pre). call (_:true). auto. call (_:true). auto.
-call (_:true). auto.  call (_:true). auto. call (_:true). auto. skip. progress.
-if. inline*. while (true). auto. auto. auto.
-seq 2 : (#pre /\ func492 = (y2_in - y1_in) * R %% P).
-ecall (submod_h y2 y1 P). inline*. wp. skip. progress. smt. smt. smt. smt. smt. smt.
-rewrite  - qqq. smt (@Int @IntDiv).
-seq 2 : (#pre /\ func500 = (x2_in - x1_in) * R %% P).
-ecall (submod_h x2 x1 P). inline*. wp. skip. progress. smt. smt. smt. smt. smt. smt.
-rewrite  - qqq. smt (@Int @IntDiv).
-pose slope_raw := (y2_in - y1_in) * (inv P (x2_in - x1_in)).
-seq 1 : (#pre /\ slope = slope_raw * R %% P).
-ecall (div_m_h (y2_in - y1_in) (x2_in - x1_in)). skip. progress. smt. smt.
-case (x2_in <> x1_in). progress.
-have : (x2_in - x1_in) %% P <> 0. smt.
-progress.
-have : (x2_in - x1_in) * R %% P <> 0.
- rewrite - dvdzE.
- case (P %| (x2_in - x1_in) * R).
-move => q.
-  have qq : P %| (x2_in - x1_in) \/ P %| R.
-  apply Euclide. auto. smt.
-elim qq. smt. apply div_fact2. smt. smt.
-smt.
-smt.
-simplify.
-     (* 
-
-y1^2 %% P = y2^2 %% P
-
-
-
-y1^2 %% P - y2^2 %% P = 0
-(y1^2 - y2^2) %% P  = 0
-y1^2 %% P = -y2^2 %% P
-(y1 - y2)(y1 + y2) %% P = 0     
-
- *)
-move => eqq.
-have : y2_in %%P = (P - y1_in) %%P.
-apply (oi y2_in y1_in). smt. smt. smt.
-have ->: y2_in ^ 2 = y2_in * y2_in. smt.
-have ->: y1_in ^ 2 = y1_in * y1_in. smt.
-rewrite H7 H8. smt().
-smt().
-smt.
-seq 1 : (#pre /\ func510 = (slope_raw * slope_raw) * R %% P).
-ecall (mul_m_h slope_raw slope_raw). skip. progress. smt. smt. smt. smt.
-seq 2 : (#pre /\ func516 = (x1_in + x2_in) * R %% P).
-ecall (addmod_h x1 x2 P). inline*. wp. skip. progress. smt. smt. smt. smt. smt. smt.
-smt(@Int @IntDiv).
-seq 2 : (#pre /\ x3 = (slope_raw * slope_raw - (x1_in + x2_in)) * R %% P).
-ecall (submod_h func510 func516 P). inline*. wp. skip. progress. smt. smt. smt. smt. smt. smt.
-rewrite - qqq. auto. smt(@Int).
-seq 2 : (#pre /\ func532 = (x1_in - (slope_raw * slope_raw - (x1_in + x2_in))) * R %% P).
-ecall (submod_h x1 x3 P). inline*. wp. skip. progress. smt. smt. smt. smt. smt. smt.
-rewrite - qqq. smt(@Int).
-pose func532_raw := (x1_in - (slope_raw * slope_raw - (x1_in + x2_in))).
-seq 1 : (#pre /\ func528 = slope_raw * func532_raw * R %% P).
-ecall (mul_m_h slope_raw func532_raw). skip. progress. smt. smt. smt. smt.
-seq 2 : (#pre /\ y3 = ((slope_raw * func532_raw) - y1_in) * R %% P).
-ecall (submod_h func528 y1 P). inline*. wp. skip. progress. smt. smt. smt. smt. smt. smt.
-rewrite - qqq. smt(@Int).
-wp.
-ecall (outof_m_h y3).
-ecall (outof_m_h x3).
-skip. progress. smt. smt. smt. smt.
-have ->: (slope_raw * slope_raw - (x1_in + x2_in)) * R %% P * inv P R %% P
- = (slope_raw * slope_raw - (x1_in + x2_in)) %% P. admit. smt.
-have ->: (slope_raw * func532_raw - y1_in) * R %% P * inv P R %% P
- = (slope_raw * func532_raw - y1_in) %% P. admit.
  smt.
-qed.
 
 
 
-
-op add_x (x y : int) =  let slope = 3 * (x ^ 2) * inv P (2 * y) in (slope ^ 2 - (2 * x)).
-op add_y (x y : int) =  let slope = 3 * (x ^ 2) * inv P (2 * y) in
-                        let x3 = add_x x y in (slope  * (x - x3) - y).
-
-lemma nosmt even_fact (n a : int) : n - a = a => even n .
+lemma ecAdd_correctness &m (x1_in y1_in x2_in y2_in : int) :
+         0 <= x1_in < P
+         /\ 0 <= y1_in < P
+         /\ 0 <= x2_in < P
+         /\ 0 <= y2_in < P
+         /\ (!pIsInfinity (x1_in, y1_in) => pointIsInCurve x1_in y1_in)
+         /\ (!pIsInfinity (x2_in, y2_in) => pointIsInCurve x2_in y2_in) =>
+    
+     Pr[ AlmostYul.main(x1_in, y1_in, x2_in, y2_in)@&m : res = ecAdd x1_in y1_in x2_in y2_in ] = 1%r.
+proof.
 progress.
-have : n = 2*a.
-rewrite - H.    smt.
-move => q. rewrite q. smt.
-qed.    
+
+case (pIsInfinity (x1_in, y1_in)).
+case (pIsInfinity (x2_in, y2_in)).
+progress.
+byphoare (_: arg = (x1_in,y1_in,x2_in,y2_in) ==> _). conseq (ecAdd_correct_1 x1_in y1_in x2_in y2_in).
+progress. smt(). smt(). smt(). smt(). smt(). auto. auto.
+
+progress.
+ have : Pr[AlmostYul.main(x1_in, y1_in, x2_in, y2_in) @ &m :
+   res = ecAdd x1_in y1_in x2_in y2_in] >= Pr[ AlmostYul.skipf()@&m : true ].
+ byequiv (_: arg{2} = (x1_in,y1_in,x2_in,y2_in) ==> _). symmetry.
+ conseq (ecAdd_correct_2 x1_in y1_in x2_in y2_in). 
+ progress. smt(). smt(). smt(). smt(). smt(). smt(). progress. smt(). auto. auto.
+ have ->: Pr[AlmostYul.skipf() @ &m : true] = 1%r. byphoare. proc. auto. auto. auto.
+ smt(@Distr).
 
 
-lemma ecAdd_correct_5 x1_in y1_in x2_in y2_in :  
- hoare[ AlmostYul.main : 
-         arg = (x1_in,y1_in,x2_in,y2_in) 
-         /\ !(x1_in = 0 /\ y1_in = 0)
-         /\ !(x2_in = 0 /\ y2_in = 0) 
-         /\ 0 <= x1_in < AlmostYUL.N 
-         /\ 0 < y1_in < AlmostYUL.N (* to be disjoint from  *)
-         /\ 0 <= x2_in < AlmostYUL.N 
-         /\ 0 < y2_in < AlmostYUL.N      
-         /\ pointIsInCurve x1_in y1_in
-         /\ pointIsInCurve x2_in y2_in
-         /\ (x1_in = x2_in /\ y1_in = y2_in)
-               ==> res = ((add_x x1_in y1_in) %% P, (add_y x1_in y1_in) %% P) ].
-proc.             
-rcondf 5. inline*. wp. skip. progress. smt().
-rcondt 5. inline*. wp. skip. progress. 
-rcondf 7. inline*. auto. smt().
-rcondt 7. inline*. wp. skip. progress.
-rcondf 9. inline*. wp. skip. progress. smt().
-rcondt 9. inline*. auto. 
-rcondf 14. inline*. auto. smt().
-rcondf 19. inline*. auto. smt().
-rcondf 24. inline*. auto. progress. rewrite /as_bool.
- have f: (AlmostYUL.N - y2{hr}) %% R = (AlmostYUL.N - y2{hr}). smt.
- rewrite f f. 
- have ->: (AlmostYUL.N - y2{hr}) %% AlmostYUL.N = (AlmostYUL.N - y2{hr}). smt.
- case (AlmostYUL.N - y2{hr} <> y2{hr});auto.
-  move => j.
-  have : even AlmostYUL.N. apply (even_fact AlmostYUL.N y2{hr}). auto.
-  smt.             
-rcondt 24. inline*. auto. progress. rewrite /as_bool.
-rcondf 33. inline*. auto. 
+case (pIsInfinity (x2_in, y2_in)).
+progress.
+ have : Pr[AlmostYul.main(x1_in, y1_in, x2_in, y2_in) @ &m :
+   res = ecAdd x1_in y1_in x2_in y2_in] >= Pr[ AlmostYul.skipf()@&m : true ].
+ byequiv (_: arg{2} = (x1_in,y1_in,x2_in,y2_in) ==> _). symmetry.
+ conseq (ecAdd_correct_3 x1_in y1_in x2_in y2_in). 
+ progress. smt(). smt(). smt(). smt(). smt(). smt(). progress. smt(). auto. auto.
+ have ->: Pr[AlmostYul.skipf() @ &m : true] = 1%r. byphoare. proc. auto. auto. auto.
+ smt(@Distr).
 
-rcondt 36. inline*. auto. progress. rewrite /as_bool.
-rcondf 63. wp. auto.
-seq 35 : (#pre). inline*. auto.
-    
-seq 2 : (#pre /\ x = x1_in * R %% P  /\ y = y1_in * R %% P). auto.
-ecall (into_m_h y1).
-ecall (into_m_h x1). 
-skip. progress. smt. smt(). smt.
-rcondf 3.  inline 2. wp.             
-ecall (pointIsInCurve_m_h x1_in y1_in). skip. progress.  rewrite /as_bool. simplify.
-have ->: y2{hr} * y2{hr} * R %% P
-  = y2{hr} * y2{hr} %% P * R %% P. smt(@IntDiv).
-rewrite H9. smt(@Int @IntDiv).
-pose x1_squared_raw := x1_in * x1_in.              
-seq 3 : (#pre /\ x1_squared = x1_squared_raw * R %% P). auto.
-ecall (mul_m_h x1_in x1_in). call (_:true);auto. call (_:true);auto. progress.
-smt. smt. smt. smt. inline 1. sp.
-seq 1 : (#pre /\ func372 = (x1_squared + x1_squared) %% P). inline*. wp. skip. progress. smt.
-seq 2 : (#pre /\ func368 = (x1_squared + (x1_squared + x1_squared)) %% P). inline*. wp. skip. progress.
-pose x:= x2{hr} * x2{hr} * R %% P.
-     have ->: (x + (x + x) %% P) %% R = (x + (x + x) %% P). smt.
-             smt(@Int @IntDiv).
-seq 2 : (#pre /\ func382 = (y1_in + y1_in) * R %% P). inline*. wp.  progress. skip. progress.
-have ->: (y2{hr} * R %% P + y2{hr} * R %% P) %% R  = (y2{hr} * R %% P + y2{hr} * R %% P) . smt.
-smt(@Int @IntDiv).  
-  
-pose slope_raw := (3 * x1_squared_raw) * (inv P (y1_in + y1_in)).             
-seq 1 : (#pre /\ slope = slope_raw * R %% P).
-ecall (div_m_h (3 * x1_in * x1_in) (y1_in + y1_in)).
-skip. progress.
-have ->: (x1_squared_raw * R %% P +
- (x1_squared_raw * R %% P + x1_squared_raw * R %% P)) %% P
-  = (x1_squared_raw * R %% P +
- (x1_squared_raw * R %% P + x1_squared_raw * R %% P) %% P) %% P. smt(@Int @IntDiv).
-have ->: (x1_squared_raw * R %% P + x1_squared_raw * R %% P) %% P
- = (x1_squared_raw * R + x1_squared_raw * R ) %% P. smt(@Int @IntDiv).
- have ->: (x1_squared_raw * R %% P + (x1_squared_raw * R + x1_squared_raw * R) %% P) %%
-P = (x1_squared_raw * R + (x1_squared_raw * R + x1_squared_raw * R)) %%
-P. smt(@Int @IntDiv). smt(@Int).
+progress.
+case (x1_in = x2_in /\ (P - y1_in) %% P = y2_in).
+move => ass.
+ have : Pr[AlmostYul.main(x1_in, y1_in, x2_in, y2_in) @ &m :
+   res = ecAdd x1_in y1_in x2_in y2_in] >= Pr[ AlmostYul.skipf()@&m : true ].
+ byequiv (_: arg{2} = (x1_in,y1_in,x2_in,y2_in) ==> _). symmetry.
+ conseq (ecAdd_correct_4 x1_in y1_in x2_in y2_in). 
+ progress. smt(). smt(). smt(). smt(). smt(). smt(). progress. smt(). smt(). auto. auto.
+ have ->: Pr[AlmostYul.skipf() @ &m : true] = 1%r. byphoare. proc. auto. auto. auto.
+ smt(@Distr).
 
-smt. smt.
 
-have ->: (y2{hr} + y2{hr}) = 2 * y2{hr}. smt().
- have : 2 * y2{hr} * R %% P <> 0. 
- (* smt(@IntDiv @Int). *)
- rewrite - dvdzE. 
- case (P %| 2 * y2{hr} * R). move => q.
- 
+progress.
+case (x1_in = x2_in /\ y1_in = y2_in).
+move => ass2.
+ have : Pr[AlmostYul.main(x1_in, y1_in, x2_in, y2_in) @ &m :
+   res = ecAdd x1_in y1_in x2_in y2_in] >= Pr[ AlmostYul.skipf()@&m : true ].
+ byequiv (_: arg{2} = (x1_in,y1_in,x2_in,y2_in) ==> _). symmetry.
+ conseq (ecAdd_correct_5 x1_in y1_in x2_in y2_in). 
+ progress. smt(). smt(). smt(). smt(). smt(). smt(). progress. smt().  
+  progress. smt(). auto.  auto.
+ have ->: Pr[AlmostYul.skipf() @ &m : true] = 1%r. byphoare. proc. auto. auto. auto.
+ smt(@Distr).
 
-  have qq : P %| 2 * y2{hr} \/ P %| R.
-  apply Euclide. auto. smt.
-  elim qq. move => zz.
-  have ww : P %| 2 \/ P %| y2{hr}.
-  apply Euclide. auto. smt.
-  elim ww. progress. apply div_fact. smt.
-  progress. apply div_fact. smt.
-  progress. apply div_fact2. smt. smt. auto.
-smt. 
-smt.
-smt. 
-seq 1 : (#pre /\ func392 = (slope_raw * slope_raw) * R %% P).
-ecall (mul_m_h slope_raw slope_raw). skip. progress. smt. smt. smt. smt.             
-seq 2 : (#pre /\ func398 = (x1_in + x1_in) * R %% P). inline*. wp. skip. progress.
-have ->: (x2{hr} + x2{hr}) * R = (x2{hr} * R + x2{hr} * R). smt. 
-have ->: (x2{hr} * R %% P + x2{hr} * R %% P) %% R 
-  = (x2{hr} * R %% P + x2{hr} * R %% P). smt.
-  smt(@Int @IntDiv).
-  
-pose x3_raw := ((slope_raw * slope_raw) - (x1_in + x1_in)).
-seq 2 : (#pre /\ x3 = x3_raw * R %% P).
-                 
-ecall (submod_h (slope_raw * slope_raw * R %% P) ((x1_in + x1_in) * R %% P) P). inline*.  wp. skip. progress.
-smt(@Int @IntDiv). smt(@Int @IntDiv). smt(@Int @IntDiv). smt. smt(@Int @IntDiv). smt(@Int @IntDiv).
-  
-have ->: (slope_raw * slope_raw - (x2{hr} + x2{hr})) * R
-              = (slope_raw * slope_raw * R - (x2{hr} + x2{hr}) * R).
-                 smt(@Int @IntDiv).
-rewrite - qqq.  auto.
-
-seq 2 : (#pre /\ func414 = (x1_in - x3_raw) * R %% P).
-ecall (submod_h x x3 P). inline*. wp. skip. progress.
-smt(@Int @IntDiv). smt(@Int @IntDiv). smt(@Int @IntDiv). smt. smt(@Int @IntDiv). smt(@Int @IntDiv).              
-smt(@Int @IntDiv). 
-
-seq 1 : (#pre /\ func410 = slope_raw * (x1_in - x3_raw) * R %% P).
-ecall (mul_m_h slope_raw (x1_in - x3_raw)). skip. progress. smt(@Int @IntDiv).
-smt(@Int @IntDiv). smt(@Int @IntDiv). smt(@Int @IntDiv).              
-
-seq 2 : (#pre /\ y3 = (slope_raw * (x1_in - x3_raw) -  (y1_in)) * R %% P).
-ecall (submod_h func410 y P). inline*. wp. skip. progress.
-smt(@Int @IntDiv). smt(@Int @IntDiv). smt(@Int @IntDiv).
-smt. smt(@Int @IntDiv). smt(@Int @IntDiv). 
-rewrite - qqq. smt(@Int).
-wp.
-ecall (outof_m_h y3).
-ecall (outof_m_h x3).
-skip. progress.
-smt(@Int @IntDiv).
-smt(@Int @IntDiv).                            
-smt(@Int @IntDiv).
-smt(@Int @IntDiv).
-have ->: x3_raw * R %% P * inv P R %% P = x3_raw %% P.
-  have ->: x3_raw * R %% P * inv P R %% P
-    = x3_raw * R %% P * (inv P R %% P) %% P. smt(@Int @IntDiv).
-   have ->: x3_raw * R %% P * (inv P R %% P) %% P = (x3_raw * R  * (inv P R)) %% P.
-   smt(@Int @IntDiv).
-   have ->: (x3_raw * R  * (inv P R)) = (x3_raw * (R  * (inv P R))). smt().
-   have ->: x3_raw * (R * inv P R) %% P = x3_raw  * ((R * inv P R) %% P )  %% P. smt(@Int @IntDiv).
-   rewrite inv_ax_opp. smt. auto.
-    
-rewrite /add_x. simplify.
-rewrite /x3_raw.
-rewrite /slope_raw.
-rewrite /x1_squared_raw.
-have ->: (x2{hr} * x2{hr}) = x2{hr} ^ 2. smt.
-congr. congr. smt.
-
-have ->: (slope_raw * (x2{hr} - x3_raw) - y2{hr}) * R %% P * inv P R %% P
-              = (slope_raw * (x2{hr} - x3_raw) - y2{hr}) %% P.
-have ->: (slope_raw * (x2{hr} - x3_raw) - y2{hr}) * R %% P * inv P R %% P
- = ((slope_raw * (x2{hr} - x3_raw) - y2{hr}) * (inv P R * R)) %% P. smt(@Int @IntDiv).
-have ->: ((slope_raw * (x2{hr} - x3_raw) - y2{hr}) * (inv P R * R)) %% P
-  = ((slope_raw * (x2{hr} - x3_raw) - y2{hr}) * ((inv P R * R) %% P)) %% P. smt(@Int @IntDiv).
-rewrite inv_ax.  simplify. smt. simplify. auto.
-              
-congr. congr.
-rewrite /add_y /add_x. simplify.
-rewrite /slope_raw.
-rewrite /x1_squared_raw.
-rewrite /x3_raw.
-rewrite /slope_raw.
-rewrite /x1_squared_raw.
-have ->: (x2{hr} * x2{hr}) = x2{hr} ^ 2. smt.
-congr.
-have ->: (3 * x2{hr} ^ 2 * inv P (y2{hr} + y2{hr}) *
-  (3 * x2{hr} ^ 2 * inv P (y2{hr} + y2{hr})) = (3 * x2{hr} ^ 2 * inv P (2 * y2{hr})) ^ 2). smt.
-smt.
+progress.
+ have : Pr[AlmostYul.main(x1_in, y1_in, x2_in, y2_in) @ &m :
+   res = ecAdd x1_in y1_in x2_in y2_in] >= Pr[ AlmostYul.skipf()@&m : true ].
+ byequiv (_: arg{2} = (x1_in,y1_in,x2_in,y2_in) ==> _). symmetry.
+ conseq (ecAdd_correct_6 x1_in y1_in x2_in y2_in). 
+ progress. smt(). smt(). smt(). smt(). smt(). smt(). progress. smt().  
+  progress. smt(). auto.  auto.
+ have ->: Pr[AlmostYul.skipf() @ &m : true] = 1%r. byphoare. proc. auto. auto. auto.
+ smt(@Distr).
 qed.
