examples/ecAdd/proofs/ecAdd_cases.ec
@@ -1,0 +1,589 @@
+require import AllCore Int IntDiv.
+require import Gcd Gcd_props.
+
+require import AlmostYUL.
+require import Montgomery_arith.
+require import EcAdd_functions.
+
+lemma nosmt even_fact (n a : int) : n - a = a => even n .
+progress.
+have : n = 2*a.
+rewrite - H.    smt.
+move => q. rewrite q. smt.
+qed.    
+
+
+lemma nosmt div_fact (a P : int) : 0 < a < P /\ 0 <= P => !(P %| a).
+progress. smt(@Int @IntDiv dvdn_le). qed.
+
+
+
+lemma nosmt div_fact2 (a P : int) : 1 < P => coprime P a => !(P %| a).
+progress.
+have ->: a = a * 1. smt().
+case (P %| a * 1);auto.
+move => q.
+have : P %| 1.
+    apply (Gauss P a 1).     auto. auto.
+apply div_fact. progress. smt().
+qed.    
+
+
+lemma nosmt qqq (a b P : int) : (a - b) %% P = (a %% P - b %% P) %% P.
+    smt(@Int @IntDiv). qed.
+
+
+lemma nosmt oi (y1 y2 : int) : 0 <= y1 < P /\ 0 <= y2 < P => y1 <> y2 => 0 < y1 + y2 => y1^2 %% P = y2^2 %% P => y1 %% P = (P - y2) %% P.
+progress.
+have fact1 : y1^2 %% P - y2^2 %% P = 0.    smt.
+have  :  (y1^2  - y2^2) %% P  = 0. rewrite qqq. rewrite fact1. auto.
+have  ->:  (y1^2  - y2^2) = (y1 - y2) * (y1 + y2). smt.
+progress.
+rewrite - dvdzE in H6.
+have fact2 : P %| (y1 + y2). apply (Gauss P _ _ H6).
+apply prime_coprime. smt. 
+have : `|y1 - y2| < P. smt(@Int).
+progress.
+case ((y1 - y2) %% P = 0). 
+move => oo.
+have : `|y1 - y2| %% P = 0. smt (@Int @IntDiv).
+progress. apply div_fact2. smt. apply prime_coprime. smt. smt.
+auto.
+have fact4 : exists k, (y1 + y2) = k * P.
+     have d :   P %| (y1 + y2) <=> exists (q : int), y1 + y2 = q * P. apply (dvdzP P (y1 + y2)).
+       elim d. progress. apply (H7 fact2).
+elim fact4. progress.
+have o1 : k = 1. smt.
+have : P = y1 + y2. smt.
+smt.
+qed.
+     
+
+
+
+lemma ecAdd_correct_0 x1_in y1_in x2_in y2_in :  
+ phoare[ AlmostYul.main : 
+         arg = (x1_in,y1_in,x2_in,y2_in)/\
+         !(x1_in < AlmostYUL.N
+         /\ y1_in < AlmostYUL.N
+         /\ x2_in < AlmostYUL.N
+         /\ y2_in < AlmostYUL.N)
+                 ==> true ] = 0%r.
+hoare. simplify.
+proc.
+rcondt 6.
+rcondf 5.
+inline*. progress. wp. skip. progress.
+smt.               
+inline*. progress. auto.
+seq 5 : (#pre /\ ret_bool = false /\ p1IsInfinity = pIsInfinity (x1,y1) /\ p2IsInfinity = pIsInfinity (x2,y2) ). inline*. progress. wp. skip. progress. smt.
+seq 2 : (#pre /\  func43 = (pIsInfinity (x1_in, y1_in) /\ !pIsInfinity  (x2_in, y2_in))). inline*. wp. skip.
+progress.   
+if.
+  seq 6 : (false).
+inline*. sp. rcondt 1. skip. progress. smt.
+while (true). auto. skip. auto. exfalso.                              
+rcondt 1. auto.
+               
+seq 2 : (#pre /\ func109 = (!pIsInfinity (x1_in, y1_in) /\ pIsInfinity  (x2_in, y2_in)) ). inline*. auto.
+if.
+  seq 6 : (false).
+inline*. sp. rcondt 1. skip. progress. smt.
+while (true). auto. skip. auto. exfalso.               
+rcondt 1. auto.
+  seq 6 : (#pre /\ !(!x1 < P \/  !y1 < P)).
+               
+seq 5 : (#pre /\ func175 = (!x1 < P \/  !y1 < P) ). inline*. auto.  progress.
+if. inline*. while (true). auto. auto. skip. progress.  
+seq 6 : (false).               
+inline*. sp. rcondt 1. skip. progress. smt.
+while (true). auto. skip. auto. exfalso.               
+qed.
+
+lemma ecAdd_correct_00 x1_in y1_in x2_in y2_in :  
+ phoare[ AlmostYul.main : 
+         arg = (x1_in,y1_in,x2_in,y2_in) /\
+      (x1_in < AlmostYUL.N
+         /\ y1_in < AlmostYUL.N
+         /\ x2_in < AlmostYUL.N
+         /\ y2_in < AlmostYUL.N) /\      
+         (((!pIsInfinity (x1_in, y1_in)) /\ (!pointIsInCurve x1_in y1_in)) \/
+         ((!pIsInfinity (x2_in, y2_in)) /\ (!pointIsInCurve x2_in y2_in)))      
+                 ==> true ] = 0%r.
+hoare. simplify.
+proc.
+seq 5 : (#pre /\ ret_bool = false). inline*.
+seq 10 : (#pre /\ ret_bool = false  /\ func17 = (pIsInfinity (x1_in, y1_in) /\ pIsInfinity (x2_in, y2_in))
+ /\  p1IsInfinity = pIsInfinity (x1_in, y1_in)
+ /\  p2IsInfinity = pIsInfinity (x2_in, y2_in)                 
+ ). wp. skip. progress.
+rcondf 1. skip. progress. smt. skip. smt.
+rcondt 1. auto.
+seq 2 : (#pre /\ func43 = (p1IsInfinity /\ !p2IsInfinity)). inline*.  wp. skip. auto.
+if.
+seq 11 : (false). admit.
+exfalso. 
+rcondt 1. auto.
+
+seq 2 : (#pre /\ func109 = (!p1IsInfinity /\ p2IsInfinity)). inline*. wp. skip. auto.
+if.
+ seq 11  : (false). admit.
+exfalso. 
+admitted.
+
+
+
+
+lemma ecAdd_correct_1 x1_in y1_in x2_in y2_in :  
+ phoare[ AlmostYul.main : 
+         arg = (x1_in,y1_in,x2_in,y2_in)  
+         /\ (x1_in = 0 /\ y1_in = 0) 
+         /\ (x2_in = 0 /\ y2_in = 0)
+                 ==> res = (0,0) ] = 1%r.
+proc. 
+rcondt 5. inline*. wp. skip. progress. 
+rcondf 7. inline*. wp. skip. progress.
+inline*. wp. auto. qed.
+
+
+lemma ecAdd_correct_2 x1_in y1_in x2_in y2_in :  
+ equiv [ AlmostYul.main ~ AlmostYul.skipf : 
+         (arg = (x1_in,y1_in,x2_in,y2_in)  
+         /\ 0 <= x2_in < AlmostYUL.N 
+         /\ 0 <= y2_in < AlmostYUL.N
+         /\ pointIsInCurve x2_in y2_in
+      
+         /\ (x1_in = 0 /\ y1_in = 0) 
+         /\ !(x2_in = 0 /\ y2_in = 0)){1}      
+                  ==> res{1} = (x2_in,y2_in) ].
+proc. 
+rcondf {1} 5. progress. inline*. wp. skip. progress. 
+rcondt {1} 5. progress. inline*. wp. skip. progress.
+rcondf {1} 8. progress. inline*. auto. sp. if. wp. sp.  auto. skip. smt().
+rcondt {1} 7. progress. inline*. wp. skip. progress.
+rcondf {1} 12. progress. inline*. wp. skip. progress.           smt().
+seq  13 0 : (#pre /\ m_x2 = x2_in * R %% P  /\ m_y2 = y2_in * R %% P){1}. auto.
+ecall {1} (into_m y2{1}).
+ecall {1} (into_m x2{1}).
+inline*. wp. skip. progress. 
+wp.
+rcondf {1} 3. progress. 
+inline AlmostYul.iszero. wp.
+ecall (pointIsInCurve_m_h x2 y2). skip. progress. rewrite /as_bool. simplify.
+rewrite /pointIsInCurve in H4.
+ have ->: y2{hr} * y2{hr} * R %% P = y2{hr} * y2{hr} %% P * R %% P.
+  smt (@Int @IntDiv).                
+  rewrite H3. smt(@IntDiv).
+call {1} (_:true ==> true). proc. auto.
+call {1} (_:true ==> true). proc. inline*. auto. skip. progress.
+qed.           
+
+
+
+lemma ecAdd_correct_3 x1_in y1_in x2_in y2_in :  
+ equiv[ AlmostYul.main ~ AlmostYul.skipf :
+         arg{1} = (x1_in,y1_in,x2_in,y2_in) 
+         /\ (0 <= x1_in < AlmostYUL.N){1}
+         /\ (0 <= y1_in < AlmostYUL.N){1}
+         /\ (pointIsInCurve x1_in y1_in){1}
+
+         /\ !(x1_in = 0 /\ y1_in = 0){1}
+         /\ (x2_in = 0 /\ y2_in = 0){1}       
+               ==> res{1} = (x1_in,y1_in){1} ].
+proc. 
+rcondf {1} 5. progress. inline*. wp. skip. progress. 
+rcondt {1} 5. progress. inline*. wp. skip. progress. 
+rcondf {1} 7. progress. inline*. auto.
+rcondt {1} 7. progress. inline*. wp. skip. progress.
+rcondt {1} 9.  progress. inline*. wp. skip. progress.       
+rcondf {1} 22.  progress. wp.  auto.
+rcondf {1} 14. progress. inline*. wp. skip. progress.        smt().
+seq {1} 15 0 : (#pre /\ m_x1 = x1_in * R %% P  /\ m_y1 = y1_in * R %% P){1}. auto.
+ecall {1} (into_m y1{1}).
+ecall {1} (into_m x1{1}).
+inline*. auto.
+wp.
+rcondf {1} 3. progress.      
+inline AlmostYul.iszero. wp.
+ecall (pointIsInCurve_m_h x1 y1). skip. progress. rewrite /as_bool. simplify.
+rewrite /pointIsInCurve in H4.
+have ->: y1{hr} * y1{hr} * R %% P
+  = y1{hr} * y1{hr} %% P * R %% P. smt(@IntDiv).
+rewrite H3. smt(@IntDiv).
+call {1} (_:true ==> true). proc. auto.
+call {1} (_:true ==> true). proc. inline*. auto.
+skip. auto.  
+qed.       
+
+lemma ecAdd_correct_4 x1_in y1_in x2_in y2_in :  
+ equiv [ AlmostYul.main ~ AlmostYul.skipf : 
+         (arg = (x1_in,y1_in,x2_in,y2_in) 
+         /\ 0 <= x1_in < AlmostYUL.N 
+         /\ 0 <= y1_in < AlmostYUL.N
+         /\ 0 <= x2_in < AlmostYUL.N 
+         /\ 0 <= y2_in < AlmostYUL.N      
+         /\ pointIsInCurve x1_in y1_in
+         /\ pointIsInCurve x2_in y2_in
+
+         /\ !(x1_in = 0 /\ y1_in = 0)
+         /\ !(x2_in = 0 /\ y2_in = 0)       
+         /\ x1_in = x2_in /\ (P - y1_in) %% P = y2){1}
+               ==> res{1} = (0,0) ].
+proc.             
+rcondf {1} 5. progress. inline*. wp. skip. progress.  smt().
+rcondt {1} 5. progress. inline*. wp. skip. progress. 
+rcondf {1} 7. progress. inline*. auto. smt().
+rcondt {1} 7. progress. inline*. wp. skip. progress.
+rcondf {1} 9. progress. inline*. wp. skip. progress. smt().
+rcondt {1} 9. progress. inline*. auto. 
+rcondf {1} 14. progress. inline*. auto. smt().
+rcondf {1} 19. progress. inline*. auto. smt().
+rcondt {1} 24. progress. inline*. auto. progress. rewrite /as_bool. smt.
+rcondf {1} 36. progress. wp. auto.
+wp.
+seq 27 0 : (#pre /\ m_x1 = x1_in * R %% P  
+               /\ m_y1 = y1_in * R %% P 
+               /\ m_x2 = x2_in * R %% P  
+               /\ m_y2 = y2_in * R %% P){1}. auto.
+ecall {1} (into_m y2{1}).
+ecall {1} (into_m x2{1}).
+ecall {1} (into_m y1{1}).
+ecall {1} (into_m x1{1}).
+inline*. auto. progress.
+rcondf {1} 6. progress.
+inline 5. inline 2. inline 5. wp.
+ecall (pointIsInCurve_m_h  x2_in y2_in).
+wp.
+ecall (pointIsInCurve_m_h  x1_in y1_in).
+skip. progress. rewrite /as_bool.
+have ->: y1{hr} * y1{hr} * R %% P = (x2{hr} * x2{hr} * x2{hr} * R + 3 * R) %% P.
+have ->: y1{hr} * y1{hr} * R %% P = y1{hr} * y1{hr} %% P * R %% P.
+smt(@Int @IntDiv).             
+rewrite  H7.  smt(@Int @IntDiv). simplify.
+have ->: (x2{hr} * x2{hr} * x2{hr} * R + 3 * R) %% P
+ = (x2{hr} * x2{hr} * x2{hr}  + 3 ) * R %% P.
+smt(@Int @IntDiv).
+have ->: (x2{hr} * x2{hr} * x2{hr}  + 3 ) * R %% P
+ = (x2{hr} * x2{hr} * x2{hr}  + 3) %% P * R %% P.
+smt(@Int @IntDiv).
+rewrite - H8. smt(@Int @IntDiv).
+inline*. auto. 
+qed.
+
+
+lemma ecAdd_correct_6 x1_in y1_in x2_in y2_in :  
+ equiv[ AlmostYul.main ~ AlmostYul.skipf : 
+         (arg = (x1_in,y1_in,x2_in,y2_in)
+         /\ 0 <= x1_in < AlmostYUL.N 
+         /\ 0 <= y1_in < AlmostYUL.N 
+         /\ 0 <= x2_in < AlmostYUL.N 
+         /\ 0 <= y2_in < AlmostYUL.N      
+         /\ pointIsInCurve x1_in y1_in
+         /\ pointIsInCurve x2_in y2_in
+
+         /\ !(x1_in = 0 /\ y1_in = 0)
+         /\ !(x2_in = 0 /\ y2_in = 0) 
+         /\ !(x1_in = x2_in /\ y1_in = y2_in)
+         /\ !(x1_in = x2_in /\ (P - y1_in) %% P = y2)){1}
+               ==> (res = (add_x' x1_in x2_in y1_in y2_in %% P, add_y' x1_in x2_in y1_in y2_in %% P)){1} ].
+proc.             
+rcondf {1} 5. progress. inline*. wp. skip. progress. smt().
+rcondt {1} 5. progress. inline*. wp. skip. progress. 
+rcondf {1} 7. progress. inline*. auto. smt().
+rcondt {1} 7. progress. inline*. wp. skip. progress.
+rcondf {1} 9. progress. inline*. wp. skip. progress. smt().
+rcondt {1} 9. progress. inline*. auto. 
+rcondf {1} 14. progress. inline*. auto. smt().
+rcondf {1} 19. progress. inline*. auto. smt().
+rcondf {1} 24. progress. inline*. auto. progress. rewrite /as_bool.
+ have f: (AlmostYUL.N - y1{hr}) %% R = (AlmostYUL.N - y1{hr}). smt.
+ rewrite f f. clear f.             
+case (x1{hr} = x2{hr}). progress.
+smt. auto.
+seq 23 0 : (#pre /\ ret_bool = false){1}. inline*. wp. auto.            
+rcondt {1} 1. progress. auto.
+rcondf {1} 10. progress.
+inline 9. inline 8. inline 7. wp. inline 6.
+inline 4. inline 1. inline 4. inline 7. sp. wp.
+ecall (submod_h 0 y2_in P). skip. progress. smt. smt. smt. smt.
+rewrite /as_bool.
+have ->: (-y2{hr}) %% P = (P - y2{hr}) %%P. smt(@Int @IntDiv).
+case (x1{hr} = x2{hr}). move => x_eq. simplify.
+have : y1{hr} %% P = (P - y2{hr}) %% P. 
+apply oi. smt. smt(). smt().
+have ->: (y1{hr} ^ 2  = y1{hr} *  y1{hr} ). smt.
+have ->: (y2{hr} ^ 2  = y2{hr} *  y2{hr} ). smt.
+rewrite H7 H8. smt().
+smt().             
+simplify. auto.                                    
+rcondf {1} 13. progress. inline*. auto.  progress. rewrite /as_bool.
+seq 12 0 : (#pre){1}. inline*. wp. auto.
+rcondt {1} 1. progress. auto.                        
+seq 4 0 : ((
+   (0 <= x1_in && x1_in < AlmostYUL.N) /\
+   (0 <= y1_in && y1_in < AlmostYUL.N) /\
+   (0 <= x2_in && x2_in < AlmostYUL.N) /\
+   (0 <= y2_in && y2_in < AlmostYUL.N) /\
+   pointIsInCurve x1_in y1_in /\
+   pointIsInCurve x2_in y2_in /\
+   ! (x1_in = 0 /\ y1_in = 0) /\
+   ! (x2_in = 0 /\ y2_in = 0) /\
+   ! (x1_in = x2_in /\ y1_in = y2_in) /\ ! (x1_in = x2_in /\ (P - y1_in) %% P = y2_in)) /\
+  ret_bool = false /\ x1 = x1_in * R %% P
+  /\ y1 = y1_in * R %% P
+ /\ x2 = x2_in * R %% P
+/\ y2 = y2_in * R %% P){1}.
+ecall {1} (into_m y2_in). 
+ecall {1} (into_m x2_in).
+ecall {1} (into_m y1_in).                          
+ecall {1} (into_m x1_in).
+skip. progress.
+rcondf {1} 6. progress. inline 5. inline 4. inline 2. wp.
+ecall (pointIsInCurve_m_h x2_in y2_in).
+wp. ecall (pointIsInCurve_m_h x1_in y1_in).
+skip. progress. rewrite /as_bool.
+have f1: y1_in * y1_in * R %% P = (x1_in * x1_in * x1_in * R + 3 * R) %% P.
+  have ->: y1_in * y1_in * R %% P = y1_in * y1_in %%P * R %% P. smt(@Int @IntDiv).
+  rewrite H7.  smt(@Int @IntDiv).
+have f2 : y2_in * y2_in * R %% P = (x2_in * x2_in * x2_in * R + 3 * R) %% P.
+  have ->: y2_in * y2_in * R %% P = y2_in * y2_in %% P * R %% P. smt(@Int @IntDiv).
+  rewrite H8. smt(@Int @IntDiv).
+smt().
+seq 5 0 : (#pre){1}.
+call {1} (_:true ==> true). proc. auto.
+call {1} (_:true ==> true). proc. auto.
+call {1} (_:true ==> true). proc. inline*. auto.
+call {1} (_:true ==> true). proc. inline*. auto.
+call {1} (_:true ==> true). proc. inline*. auto.
+skip. progress.
+seq 2 0 : (#pre /\ func492 = (y2_in - y1_in) * R %% P){1}.
+ecall {1} (submod y2{1} y1{1} P). inline*. wp. skip. progress. smt. smt. smt. smt. smt. smt.
+rewrite  - qqq. smt (@Int @IntDiv).
+seq 2 0 : (#pre /\ func500 = (x2_in - x1_in) * R %% P){1}.
+ecall {1} (submod x2{1} x1{1} P). inline*. wp. skip. progress. smt. smt. smt. smt. smt. smt.
+rewrite  - qqq. smt (@Int @IntDiv).
+pose slope_raw := (y2_in - y1_in) * (inv P (x2_in - x1_in)).
+seq 1 0 : (#pre /\ slope = slope_raw * R %% P){1}.
+ecall {1} (div_m (y2_in - y1_in) (x2_in - x1_in)). skip. progress. smt. smt.
+case (x2_in <> x1_in). progress.
+have : (x2_in - x1_in) %% P <> 0. smt.
+progress.
+have : (x2_in - x1_in) * R %% P <> 0.
+ rewrite - dvdzE.
+ case (P %| (x2_in - x1_in) * R).
+move => q.
+  have qq : P %| (x2_in - x1_in) \/ P %| R.
+  apply Euclide. auto. smt.
+elim qq. smt. apply div_fact2. smt. smt.
+smt.
+smt.
+simplify.
+move => eqq.
+have : y2_in %%P = (P - y1_in) %%P.
+apply (oi y2_in y1_in). smt. smt. smt.
+have ->: y2_in ^ 2 = y2_in * y2_in. smt.
+have ->: y1_in ^ 2 = y1_in * y1_in. smt.
+rewrite H7 H8. smt().
+smt().
+smt.
+seq 1 0 : (#pre /\ func510 = (slope_raw * slope_raw) * R %% P){1}.
+ecall {1} (mul_m slope_raw slope_raw). skip. progress. smt. smt. smt. smt.
+seq 2 0 : (#pre /\ func516 = (x1_in + x2_in) * R %% P){1}.
+ecall {1} (addmod x1{1} x2{1} P). inline*. wp. skip. progress. smt. smt. smt. smt. smt. smt. smt(@Int @IntDiv).
+seq 2 0 : (#pre /\ x3 = (slope_raw * slope_raw - (x1_in + x2_in)) * R %% P){1}.
+ecall {1} (submod func510{1} func516{1} P). inline*. wp. skip. progress. smt. smt. smt. smt. smt. smt.
+rewrite - qqq. auto. smt(@Int).
+seq 2 0 : (#pre /\ func532 = (x1_in - (slope_raw * slope_raw - (x1_in + x2_in))) * R %% P){1}.
+ecall {1} (submod x1{1} x3{1} P). inline*. wp. skip. progress. smt. smt. smt. smt. smt. smt.
+rewrite - qqq. smt(@Int).
+pose func532_raw := (x1_in - (slope_raw * slope_raw - (x1_in + x2_in))).
+seq 1 0 : (#pre /\ func528 = slope_raw * func532_raw * R %% P){1}.
+ecall {1} (mul_m slope_raw{1} func532_raw{1}). skip. progress. smt. smt. smt. smt.
+seq 2 0 : (#pre /\ y3 = ((slope_raw * func532_raw) - y1_in) * R %% P){1}.
+ecall {1} (submod func528{1} y1{1} P). inline*. wp. skip. progress. smt. smt. smt. smt. smt. smt.
+rewrite - qqq. smt(@Int).
+wp.
+ecall {1} (outof_m y3{1}).
+ecall {1} (outof_m x3{1}).
+skip. progress. smt. smt. smt. smt.
+have ->: (slope_raw * slope_raw - (x1_in + x2_in)) * R %% P * inv P R %% P
+ = (slope_raw * slope_raw - (x1_in + x2_in)) %% P.
+have ->: (slope_raw * slope_raw - (x1_in + x2_in)) * R %% P * inv P R %% P
+ = (slope_raw * slope_raw - (x1_in + x2_in)) * R * inv P R %% P.
+smt(@Int @IntDiv).
+have ->:  (slope_raw * slope_raw - (x1_in + x2_in)) * R * inv P R %% P
+  = (slope_raw * slope_raw - (x1_in + x2_in)) * (R * inv P R) %% P. smt().
+have ->:   (slope_raw * slope_raw - (x1_in + x2_in)) * (R * inv P R) %% P
+  = (slope_raw * slope_raw - (x1_in + x2_in)) * ((R * inv P R) %% P) %% P.
+smt(@Int @IntDiv). rewrite inv_ax_opp.   smt. simplify. auto.
+smt.
+have ->: (slope_raw * func532_raw - y1_in) * R %% P * inv P R %% P
+ = (slope_raw * func532_raw - y1_in) * (R * inv P R) %% P.
+smt(@Int @IntDiv).
+have ->: (slope_raw * func532_raw - y1_in) * (R * inv P R) %% P =
+ (slope_raw * func532_raw - y1_in) * (R * inv P R %%P) %% P.
+smt(@Int @IntDiv).
+rewrite inv_ax_opp. smt. simplify.
+ smt.
+qed.
+
+
+
+lemma ecAdd_correct_5 x1_in y1_in x2_in y2_in :  
+ equiv [ AlmostYul.main ~ AlmostYul.skipf  : 
+         (arg = (x1_in,y1_in,x2_in,y2_in) 
+         /\ 0 <= x1_in < AlmostYUL.N 
+         /\ 0 <= y1_in < AlmostYUL.N (* to be disjoint from  *)
+         /\ 0 <= x2_in < AlmostYUL.N 
+         /\ 0 <= y2_in < AlmostYUL.N      
+         /\ pointIsInCurve x1_in y1_in
+         /\ pointIsInCurve x2_in y2_in
+      
+         /\ !(x1_in = 0 /\ y1_in = 0)
+         /\ !(x2_in = 0 /\ y2_in = 0)       
+         /\ (x1_in = x2_in /\ y1_in = y2_in)){1}
+         /\ !(x1_in = x2_in /\ (P - y1_in) %% P = y2){1}
+               ==> res{1} = ((add_x x1_in y1_in){1} %% P, (add_y x1_in y1_in){1} %% P) ].
+proc.             
+rcondf {1} 5. progress. inline*. wp. skip. progress. smt().
+rcondt  {1} 5. progress. inline*. wp. skip. progress. 
+rcondf  {1} 7. progress. inline*. auto. smt().
+rcondt {1} 7. progress. inline*. wp. skip. progress.
+rcondf {1} 9. progress. inline*. wp. skip. progress. smt().
+rcondt {1} 9. progress. inline*. auto. 
+rcondf {1} 14. progress. inline*. auto. smt().
+rcondf {1} 19. progress. inline*. auto. smt().
+rcondf {1} 24. progress. inline*. auto. progress. rewrite /as_bool.
+ have f: (AlmostYUL.N - y2{hr}) %% R = (AlmostYUL.N - y2{hr}). smt.
+ rewrite f f. 
+ have ->: (AlmostYUL.N - y2{hr}) %% AlmostYUL.N = (AlmostYUL.N - y2{hr}). smt.
+ case (AlmostYUL.N - y2{hr} <> y2{hr});auto.
+  move => j.
+  have : even AlmostYUL.N. apply (even_fact AlmostYUL.N y2{hr}). auto.
+  smt.             
+rcondt {1} 24. progress. inline*. auto. progress. rewrite /as_bool.
+rcondf {1} 33. progress. inline*. auto. 
+rcondt {1} 36. progress. inline*. auto. progress. rewrite /as_bool.
+rcondf {1} 63. progress. wp. auto.
+seq 35 0 : (#pre). inline*. auto.    
+seq 2 0 : (#pre /\ x = x1_in * R %% P  /\ y = y1_in * R %% P){1}. auto.
+ecall {1} (into_m y1{1}).
+ecall {1} (into_m x1{1}). 
+skip. progress. 
+rcondf {1} 3. progress.  inline 2. wp.             
+ecall  (pointIsInCurve_m_h x1_in y1_in).
+skip. progress.  rewrite /as_bool. simplify.
+have ->: y2{hr} * y2{hr} * R %% P
+  = y2{hr} * y2{hr} %% P * R %% P. smt(@IntDiv).
+rewrite H8. smt(@Int @IntDiv).
+pose x1_squared_raw := x1_in * x1_in.              
+seq 3 0 : (#pre /\ x1_squared = x1_squared_raw * R %% P){1}. auto.
+ecall {1} (mul_m x1_in x1_in). call {1} (_:true ==> true). proc. auto. call {1} (_:true ==> true). proc. inline*. auto. skip. 
+smt.  inline {1} 1. sp.
+seq 1 0 : (#pre /\ func372 = (x1_squared + x1_squared) %% P){1}. inline*. wp. skip. progress. smt.
+seq 2 0 : (#pre /\ func368 = (x1_squared + (x1_squared + x1_squared)) %% P){1}. inline*. wp. skip. progress.
+pose x:= x2{1} * x2{1} * R %% P.
+     have ->: (x + (x + x) %% P) %% R = (x + (x + x) %% P). smt.
+             smt(@Int @IntDiv).
+seq 2 0 : (#pre /\ func382 = (y1_in + y1_in) * R %% P){1}. inline*. wp.  progress. skip. progress.
+have ->: (y2{1} * R %% P + y2{1} * R %% P) %% R  = (y2{1} * R %% P + y2{1} * R %% P) . smt.
+smt(@Int @IntDiv).    
+pose slope_raw := (3 * x1_squared_raw) * (inv P (y1_in + y1_in)).             
+seq 1 0 : (#pre /\ slope = slope_raw * R %% P){1}.
+ecall {1} (div_m (3 * x1_in * x1_in) (y1_in + y1_in)).
+skip. progress.
+have ->: (x1_squared_raw * R %% P +
+ (x1_squared_raw * R %% P + x1_squared_raw * R %% P)) %% P
+  = (x1_squared_raw * R %% P +
+ (x1_squared_raw * R %% P + x1_squared_raw * R %% P) %% P) %% P. smt(@Int @IntDiv).
+have ->: (x1_squared_raw * R %% P + x1_squared_raw * R %% P) %% P
+ = (x1_squared_raw * R + x1_squared_raw * R ) %% P. smt(@Int @IntDiv).
+ have ->: (x1_squared_raw * R %% P + (x1_squared_raw * R + x1_squared_raw * R) %% P) %%
+P = (x1_squared_raw * R + (x1_squared_raw * R + x1_squared_raw * R)) %%
+P. smt(@Int @IntDiv). smt(@Int).
+smt. smt.
+have ->: (y2{1} + y2{1}) = 2 * y2{1}. smt().
+ have : 2 * y2{1} * R %% P <> 0. 
+ (* smt(@IntDiv @Int). *)
+ rewrite - dvdzE. 
+ case (P %| 2 * y2{1} * R). move => q.
+  have qq : P %| 2 * y2{1} \/ P %| R.
+  apply Euclide. auto. smt.
+  elim qq. move => zz.
+  have ww : P %| 2 \/ P %| y2{1}.
+  apply Euclide. auto. smt.
+  elim ww. progress. apply div_fact. smt.
+  progress. apply div_fact. smt.
+  progress. apply div_fact2. smt. smt. auto.
+smt. 
+smt.
+smt. 
+seq 1 0 : (#pre /\ func392 = (slope_raw * slope_raw) * R %% P){1}.
+ecall {1} (mul_m slope_raw slope_raw). skip. progress. smt. smt. smt. smt.             
+seq 2 0 : (#pre /\ func398 = (x1_in + x1_in) * R %% P){1}. inline*. wp. skip. progress.
+have ->: (x2{1} + x2{1}) * R = (x2{1} * R + x2{1} * R). smt. 
+have ->: (x2{1} * R %% P + x2{1} * R %% P) %% R 
+  = (x2{1} * R %% P + x2{1} * R %% P). smt.
+  smt(@Int @IntDiv).
+  pose x3_raw := ((slope_raw * slope_raw) - (x1_in + x1_in)).
+seq 2 0 : (#pre /\ x3 = x3_raw * R %% P){1}.                 
+ecall {1} (submod (slope_raw * slope_raw * R %% P) ((x1_in + x1_in) * R %% P) P). inline*.  wp. skip. progress.
+smt(@Int @IntDiv). smt(@Int @IntDiv). smt(@Int @IntDiv). smt. smt(@Int @IntDiv). smt(@Int @IntDiv).  
+have ->: (slope_raw * slope_raw - (x2{1} + x2{1})) * R
+              = (slope_raw * slope_raw * R - (x2{1} + x2{1}) * R).
+                 smt(@Int @IntDiv).
+rewrite - qqq.  auto.
+seq 2 0 : (#pre /\ func414 = (x1_in - x3_raw) * R %% P){1}.
+ecall {1} (submod x{1} x3{1} P). inline*. wp. skip. progress.
+smt(@Int @IntDiv). smt(@Int @IntDiv). smt(@Int @IntDiv). smt. smt(@Int @IntDiv). smt(@Int @IntDiv).              
+smt(@Int @IntDiv). 
+seq 1 0 : (#pre /\ func410 = slope_raw * (x1_in - x3_raw) * R %% P){1}.
+ecall {1} (mul_m slope_raw (x1_in - x3_raw)). skip. progress. smt(@Int @IntDiv).
+smt(@Int @IntDiv). smt(@Int @IntDiv). smt(@Int @IntDiv).              
+seq 2 0 : (#pre /\ y3{1} = (slope_raw * (x1_in - x3_raw) -  (y1_in)) * R %% P).
+ecall {1} (submod func410{1} y{1} P). inline*. wp. skip. progress.
+smt(@Int @IntDiv). smt(@Int @IntDiv). smt(@Int @IntDiv).
+smt. smt(@Int @IntDiv). smt(@Int @IntDiv). 
+rewrite - qqq. smt(@Int).
+wp.
+ecall {1} (outof_m y3{1}).
+ecall {1} (outof_m x3{1}).
+skip. progress.
+smt(@Int @IntDiv).
+smt(@Int @IntDiv).                            
+smt(@Int @IntDiv).
+smt(@Int @IntDiv).
+have ->: x3_raw * R %% P * inv P R %% P = x3_raw %% P.
+  have ->: x3_raw * R %% P * inv P R %% P
+    = x3_raw * R %% P * (inv P R %% P) %% P. smt(@Int @IntDiv).
+   have ->: x3_raw * R %% P * (inv P R %% P) %% P = (x3_raw * R  * (inv P R)) %% P.
+   smt(@Int @IntDiv).
+   have ->: (x3_raw * R  * (inv P R)) = (x3_raw * (R  * (inv P R))). smt().
+   have ->: x3_raw * (R * inv P R) %% P = x3_raw  * ((R * inv P R) %% P )  %% P. smt(@Int @IntDiv).
+   rewrite inv_ax_opp. smt. auto.
+    rewrite /add_x. simplify.
+rewrite /x3_raw.
+rewrite /slope_raw.
+rewrite /x1_squared_raw.
+have ->: (x2{1} * x2{1}) = x2{1} ^ 2. smt.
+congr. congr. smt.
+have ->: (slope_raw * (x2{1} - x3_raw) - y2{1}) * R %% P * inv P R %% P
+              = (slope_raw * (x2{1} - x3_raw) - y2{1}) %% P.
+have ->: (slope_raw * (x2{1} - x3_raw) - y2{1}) * R %% P * inv P R %% P
+ = ((slope_raw * (x2{1} - x3_raw) - y2{1}) * (inv P R * R)) %% P. smt(@Int @IntDiv).
+have ->: ((slope_raw * (x2{1} - x3_raw) - y2{1}) * (inv P R * R)) %% P
+  = ((slope_raw * (x2{1} - x3_raw) - y2{1}) * ((inv P R * R) %% P)) %% P. smt(@Int @IntDiv).
+rewrite inv_ax.  simplify. smt. simplify. auto.              
+congr. congr.
+rewrite /add_y /add_x. simplify.
+rewrite /slope_raw.
+rewrite /x1_squared_raw.
+rewrite /x3_raw.
+rewrite /slope_raw.
+rewrite /x1_squared_raw.
+have ->: (x2{1} * x2{1}) = x2{1} ^ 2. smt.
+congr.
+have ->: (3 * x2{1} ^ 2 * inv P (y2{1} + y2{1}) *
+  (3 * x2{1} ^ 2 * inv P (y2{1} + y2{1})) = (3 * x2{1} ^ 2 * inv P (2 * y2{1})) ^ 2). smt.
+smt.
+qed.
